src/Zulib/verify.sh
@@ -4,6 +4,6 @@ mono ../../../FStar/bin/fstar.exe \
      --smt ../../packages/zen_z3_linux/output/z3-linux \
      --prims fstar/prims.fst \
      --no_default_includes \
-     --include ~/Dev/zenprotocol/src/Zulib/fstar \
+     --include ~/git/zenprotocol/src/Zulib/fstar \
      --cache_checked_modules \
      $@
